Change files

Leroy/Fixpoints.lean
@@ -9,39 +9,39 @@ import Init.Data.List.Pairwise
 import Init.Data.List.Sublist
 import Init.Data.List.Basic
 
-
 universe u
 
 set_option grind.warning false
-
-section Fixpoints
 
 @[grind] class OrderStruct (α : Sort u) where
   eq : α → α → Prop
   le : α → α → Prop
   beq : α → α → Bool
-  beq_true : ∀ x y : α, beq x y = true → eq x y
-  beq_false : ∀ x y : α, beq x y = false → ¬ eq x y
-  F : α → α
-  F_mon: ∀ x y, le x y -> le (F x) (F y)
   le_trans: ∀ x y z, le x y -> le y z -> le x z
-  bot : α
-  bot_smallest : ∀ x, le bot x
+  beq_true' : ∀ x y : α, beq x y = true → eq x y
+  beq_false' : ∀ x y : α, beq x y = false → ¬ eq x y
+  gt_wf : WellFounded (fun x y : α => le y x ∧ ¬eq y x)
 open OrderStruct
 
-@[grind] def gt {α : Sort u} [OrderStruct α] (x y : α) := le y x ∧ ¬eq y x
+@[grind] def gt {α : Sort u} [OrderStruct α] (x y : α) : Prop := le y x ∧ ¬eq y x
 
-@[grind] class WellFoundedOrderStruct (α : Sort u) extends OrderStruct α where
-  gt_wf : WellFounded (@gt α _)
+def gt_well_founded {α : Sort u} [OrderStruct α] : WellFounded (gt : α → α → Prop) := by apply @gt_wf
 
-variable ( α : Sort u ) [inst:  WellFoundedOrderStruct α]
-open WellFoundedOrderStruct
+class OrderWithBot (α : Sort u) extends OrderStruct α where
+  bot : α
+  bot_smallest : ∀ x, le bot x
 
-instance : WellFoundedRelation α  where
-  rel := gt
-  wf := gt_wf
+class Monotone (α : Sort u) (F : α → α) [OrderStruct α] where
+  F_mon : ∀ {x y : α}, le x y → le (F x) (F y)
 
-theorem fixpoint_exists_1: ∃ x : α, eq x (F x) := by
+open Monotone
+
+section FixpointExistence
+
+variable (α : Sort u) (F : α → α) [OrderWithBot α]
+
+open OrderStruct OrderWithBot
+theorem fixpoint_exists_1 [Monotone α F] : ∃ x : α, eq x (F x) := by
   have REC : forall x : α, le x (F x) -> exists y : α , eq y (F y) := by
     intro x
     induction x using @WellFounded.induction α gt gt_wf
@@ -50,28 +50,44 @@ theorem fixpoint_exists_1: ∃ x : α, eq x (F x) := by
       by_cases (beq x (F x))
       case pos isTrue =>
         exists x
-        grind [OrderStruct.beq_true]
+        grind [beq_true']
       case neg isFalse =>
-        specialize ih (F x)
-        grind [OrderStruct.beq_false, gt, OrderStruct.F_mon]
-  specialize REC bot
+        apply ih (F x)
+        . constructor
+          . exact h
+          . apply beq_false'
+            grind
+        . exact F_mon h
+  specialize REC
   apply REC
   apply bot_smallest
 
-@[grind] def iterate (x : α) (PRE: le x (F x)) (SMALL: forall z, le (F z) z -> le x z) : α :=
-  if beq x (F x) then x else iterate (F x) (by apply OrderStruct.F_mon; exact PRE) (by intro z hyp; specialize SMALL z hyp; apply le_trans; apply F_mon; exact SMALL; exact hyp)
-termination_by x
-decreasing_by
-  rename_i h
-  unfold gt
-  grind [OrderStruct.beq_false]
+end FixpointExistence
 
-@[grind] theorem iterate_correct (x : α) (PRE: le x (F x)) (SMALL: forall z, le (F z) z -> le x z) (heq : y = iterate _ x PRE SMALL ) : eq y (F y) ∧ ∀ z, le (F z) z → le y z := by
+section Iterate
+
+variable (α : Sort u) [inst : OrderStruct α] (F : α → α) [Monotone α F]
+
+open OrderStruct
+
+instance : WellFoundedRelation α  where
+  rel := gt
+  wf := gt_wf
+
+@[grind] def iterate (x : α) (PRE: le x (F x)) (SMALL: forall z, le (F z) z -> le x z) : α :=
+  if beq x (F x) then x else iterate (F x) (by apply F_mon; exact PRE) (by intro z hyp; specialize SMALL z hyp; apply le_trans; apply F_mon; exact SMALL; exact hyp)
+  termination_by x
+  decreasing_by
+    grind [beq_false']
+
+#check iterate
+
+@[grind] theorem iterate_correct (x : α) (PRE: le x (F x)) (SMALL: forall z, le (F z) z -> le x z) (heq : y = iterate _ F x PRE SMALL ) : eq y (F y) ∧ ∀ z, le (F z) z → le y z := by
   fun_induction iterate
   case case1 x' PRE SMALL isTrue  =>
     constructor
     . rw [←heq] at PRE
-      grind [OrderStruct.beq_true]
+      grind [beq_true']
     . intro z hyp
       specialize SMALL z hyp
       grind
@@ -79,28 +95,35 @@ decreasing_by
     have := @ih heq
     grind
 
-@[grind] def fixpoint' : α := iterate α bot (by apply bot_smallest) (by intro z pre; apply bot_smallest)
+end Iterate
 
-theorem fixpoint_correct : inst.eq (@fixpoint' α _) (F (@fixpoint' _ _)) /\ forall z : α , le (F z) z -> le (@fixpoint' _ _) z := by
-  unfold fixpoint'
-  have PRE : inst.le (bot) (F bot) := by apply bot_smallest
-  have SMALL : ∀ z, le (F z) z -> inst.le bot z := by
-    intro z hyp
-    apply le_trans
+section Fixpoint
+open OrderWithBot
+variable {α : Sort u} [i : OrderWithBot α] (F : α → α) [Monotone α F]
+
+@[grind] def fixpoint' : α := iterate α F bot (by apply bot_smallest) (by grind [bot_smallest])
+
+theorem fixpoint_correct :
+  eq (fixpoint' F) (F (fixpoint' F)) ∧ ∀ z : α, le (F z) z → le (fixpoint' F) z := by
+    unfold fixpoint'
+    apply iterate_correct
     rotate_left
-    . exact hyp
+    . exact bot
     . apply bot_smallest
-  have := @iterate_correct α inst (iterate α bot PRE SMALL) bot PRE SMALL (rfl)
-  grind
+    . grind [bot_smallest]
+    . rfl
+end Fixpoint
 
-end Fixpoints
+section Constprop
+
+open Std.HashMap
 
 @[grind] def Eq' (S1 S2 : Store) : Prop := Equal S1 S2
 
 def Eq'_sym : ∀ S1 S2, Eq' S1 S2 → Eq' S2 S1 := by
   intro S1 S2 hyp
   unfold Eq' Equal at *
-  grind [Std.HashMap.Equiv.symm]
+  grind [Equiv.symm]
 
 @[grind] theorem Equal_Eq' : ∀ S1 S2, (Equal S1 S2 == true) → Eq' S1 S2 := by grind
 
@@ -112,7 +135,7 @@ def Eq'_sym : ∀ S1 S2, Eq' S1 S2 → Eq' S2 S1 := by
   intro x n heq2
   unfold Eq' Equal  at heq
   simp at *
-  grind [Std.HashMap.Equiv.getElem?_eq]
+  grind [Equiv.getElem?_eq]
 
 @[grind] theorem Le_trans : ∀ S1 S2 S3, Le S1 S2 → Le S2 S3 → Le S1 S3 := by grind
 
@@ -126,7 +149,7 @@ theorem hash_set_incl_size_leq (S1 S2 : Store) : Le S2 S1 → List.Subperm (S1.t
   apply List.subperm_of_subset
   . apply List.Pairwise.imp
     rotate_left
-    . exact Std.HashMap.distinct_keys_toList
+    . exact distinct_keys_toList
     . grind
   . intro (k,v) mem
     specialize LE k v (by grind)
@@ -137,7 +160,7 @@ theorem hash_set_incl_size_leq (S1 S2 : Store) : Le S2 S1 → List.Subperm (S1.t
   Le T S ->
   S.size <= T.size ∧ (S.size = T.size → Equal S T) := by
     intro S T hyp
-    have size_eq : ∀ (S : Store), S.size = S.toList.length := by grind [Std.HashMap.length_toList]
+    have size_eq : ∀ (S : Store), S.size = S.toList.length := by grind [length_toList]
     rw [size_eq S, size_eq T]
     constructor
     case left =>
@@ -145,7 +168,7 @@ theorem hash_set_incl_size_leq (S1 S2 : Store) : Le S2 S1 → List.Subperm (S1.t
     case right =>
       intro eqLen
       unfold Equal
-      apply Std.HashMap.Equiv.of_toList_perm
+      apply Equiv.of_toList_perm
       apply List.Subperm.perm_of_length_le (hash_set_incl_size_leq S T hyp)
       grind
 
@@ -175,76 +198,102 @@ theorem Gt_wf : WellFounded Gt := by
   apply @Subrelation.wf Store (InvImage Nat.lt (fun x : Store => x.size)) Gt subrel
   exact InvImage.wf (fun x : Store => x.size) (Nat.lt_wfRel.wf)
 
+open OrderStruct
 
--- Section FIXPOINT_JOIN.
+noncomputable instance : OrderStruct Store where
+  eq := Equal
+  le := Le
+  beq (S1 S2 : Store) :=  Decidable.decide (Equal S1 S2)
+  le_trans := Le_trans
+  beq_true' := by grind
+  beq_false' := by grind
+  gt_wf := Gt_wf
+end Constprop
 
--- Variable Init: Store.
--- Variable F: Store -> Store.
--- Hypothesis F_incr: Increasing F.
+section FixpointJoin
+variable (Init : Store)
+variable (F : Store → Store) [Monotone Store F]
 
--- instance : WellFoundedOrderStruct Store where
---   eq := Eq'
---   le := Le
---   beq := fun x y => decide (Equal x y)
---   beq_true := fun x y hyp => Equal_Eq' x y (by grind)
---   beq_false := fun x y hyp => Equal_nEq x y (by grind)
---   bot := sorry
---   bot_smallest := sorry
---   F := sorry
---   F_mon := sorry
---   le_trans := Le_trans
---   gt_wf := Gt_wf
+instance : Monotone Store (fun x => Join Init (F x)) where
+  F_mon := by
+    intro x y le
+    unfold OrderStruct.le at *
+    unfold instOrderStructStore at *
+    simp at *
+    unfold Le at *
+    intro z n isSome
+    have ⟨ h1, h2 ⟩:= (Join_characterization Init (F y) z n).1 isSome
+    apply (Join_characterization (Init) (F x) z n).2
+    constructor
+    . exact h1
+    . apply @F_mon _ _ _ _ _ y le
+      exact h2
 
+noncomputable def fixpoint_join : Store := by
+  have := iterate Store (fun x => Join Init (F x)) Init (by apply Le_Join_l)
+  apply this
+  dsimp
+  intro z hyp
+  unfold le instOrderStructStore
+  dsimp
+  unfold Le
+  intro x n hyp2
+  specialize hyp x n hyp2
+  grind
 
--- def fixpoint_join (Init : Store) (F : Store → Store) (F_incr : Increasing F) : Store := by
---   have := @iterate Store
+theorem fixpoint_join_eq: Eq' (Join Init (F (fixpoint_join Init F) )) (fixpoint_join Init F) := by
+  generalize heq1 : fixpoint_join Init F = t
+  apply Eq'_sym
+  simp [fixpoint_join] at *
+  have := (@iterate_correct Store _ (fun x => Join Init (F x)) _ ?_ ?_ ?_ ?_ ?_ ).1
+  unfold Eq'
+  . exact this
+  . exact Init
+  . dsimp
+    apply Le_Join_l
+  . intro z hyp
+    unfold le instOrderStructStore
+    dsimp
+    unfold Le
+    intro x n hyp2
+    specialize hyp x n hyp2
+    grind
+  . rw [heq1]
 
--- Program Definition fixpoint_join : Store :=
---   iterate Store Eq Equal Equal_Eq Equal_nEq Le Le_trans Gt_wf
---           (fun x => Join Init (F x)) _ Init _ _.
--- Next Obligation.
---   unfold Le; intros.
---   apply Join_characterization in H0. destruct H0 as [FIND1 FIND2].
---   apply Join_characterization. split; auto. apply (F_incr _ _ H). auto.
--- Qed.
--- Next Obligation.
---   apply Le_Join_l.
--- Qed.
--- Next Obligation.
---   eapply Le_trans. apply Le_Join_l. eauto.
--- Qed.
+theorem fixpoint_join_sound : Le Init (fixpoint_join Init F) /\ Le (F (fixpoint_join Init F)) (fixpoint_join Init F) := by
+  have LE : Le (Join Init (F (fixpoint_join Init F))) (fixpoint_join Init F) := by
+    apply Eq_Le
+    apply fixpoint_join_eq
+  constructor
+  . apply Le_trans
+    rotate_left
+    . exact LE
+    . apply Le_Join_l
+  . apply Le_trans
+    rotate_left
+    . exact LE
+    . apply Le_Join_r
 
--- Lemma fixpoint_join_eq:
---   Eq (Join Init (F fixpoint_join)) fixpoint_join.
--- Proof.
---   apply Eq_sym. unfold fixpoint_join.
---   destruct iterate as (X & EQ & SMALL). auto.
--- Qed.
+theorem fixpoint_join_smallest:
+  forall S, Le (Join Init (F S)) S -> Le (fixpoint_join Init F) S := by
+    intro S LE
+    unfold fixpoint_join
+    dsimp
+    have := (@iterate_correct Store _ (fun x => Join Init (F x)) _ (fixpoint_join Init F) Init (?_) ?_ ?_).2 S LE
+    exact this
+    . dsimp
+      apply Le_Join_l
+    . intro z hyp
+      unfold le instOrderStructStore
+      dsimp
+      unfold Le
+      intro x n hyp2
+      specialize hyp x n hyp2
+      grind
+    . unfold fixpoint_join
+      dsimp
 
--- Lemma fixpoint_join_sound:
---   Le Init fixpoint_join /\ Le (F fixpoint_join) fixpoint_join.
--- Proof.
---   assert (LE: Le (Join Init (F fixpoint_join)) fixpoint_join).
---   { apply Eq_Le. apply fixpoint_join_eq. }
---   split.
--- - eapply Le_trans. apply Le_Join_l. eauto.
--- - eapply Le_trans. apply Le_Join_r. eauto.
--- Qed.
-
--- Lemma fixpoint_join_smallest:
---   forall S, Le (Join Init (F S)) S -> Le fixpoint_join S.
--- Proof.
---   unfold fixpoint_join. destruct iterate as (X & EQ & SMALL).
---   auto.
--- Qed.
-
--- End FIXPOINT_JOIN.
-
--- (** Now we can try to use the [fixpoint_join] function above in the [Cexec]
---   static analyzer.  But we are in for a surprise!
--- *)
-
-theorem Join_increasing:
+@[grind] theorem Join_increasing:
   forall S1 S2 S3 S4,
   Le S1 S2 -> Le S3 S4 -> Le (Join S1 S3) (Join S2 S4) := by
     intros
@@ -255,7 +304,7 @@ theorem Join_increasing:
     intro S1 S2 LE a
     induction a <;> grind
 
-theorem Beval_increasing : ∀ S1 S2, Le S1 S2 ->
+@[grind] theorem Beval_increasing : ∀ S1 S2, Le S1 S2 ->
   forall b n, Beval S2 b = .some n -> Beval S1 b = .some n := by
     intro S1 S2 LE b
     induction b
@@ -271,53 +320,103 @@ theorem Update_increasing:
   Le (Update x (Aeval S1 a) S1) (Update x (Aeval S2 a) S2) := by
     intros; grind
 
+end FixpointJoin
 
--- Lemma fixpoint_Join_increasing:
---   forall F (F_incr: Increasing F) S1 S2,
---   Le S1 S2 -> Le (fixpoint_join S1 F F_incr) (fixpoint_join S2 F F_incr).
--- Proof.
---   intros. apply fixpoint_join_smallest.
---   set (fix2 := fixpoint_join S2 F F_incr).
---   assert (Le (Join S2 (F fix2)) fix2) by (apply Eq_Le; apply fixpoint_join_eq).
---   eapply Le_trans; eauto.
---   apply Join_increasing; auto. unfold Le; auto.
--- Qed.
+noncomputable instance wrapper (F : Store → Store) (F_mon : ∀ x y, le x y → le (F x) (F y)) : Monotone Store F where
+  F_mon := by grind
 
--- (** At long last, we can define [Cexec] while at the same time showing that
---   it is increasing. *)
+noncomputable def fixpoint_join' (S : Store) (F: Store → Store) (F_mon : ∀ x y, le x y → le (F x) (F y)) := by
+  have := wrapper F (by grind)
+  exact fixpoint_join S F
 
--- Program Fixpoint Cexec (c: com) : { F: Store -> Store | Increasing F } :=
---   match c with
---   | SKIP => fun S => S
---   | ASSIGN x a => fun S => Update x (Aeval S a) S
---   | SEQ c1 c2 => compose (Cexec c2) (Cexec c1)
---   | IFTHENELSE b c1 c2 =>
---       fun S =>
---       match Beval S b return _ with
---       | Some true => Cexec c1 S
---       | Some false => Cexec c2 S
---       | None => Join (Cexec c1 S) (Cexec c2 S)
---       end
---   | WHILE b c1 =>
---       fun S => fixpoint_join S (fun S => Cexec c1 S) _
---   end.
--- Next Obligation.
---   unfold Increasing. auto.
--- Defined.
--- Next Obligation.
---   intros y z LE. apply Update_increasing; auto.
--- Defined.
--- Next Obligation.
---   intros y z LE. unfold compose. auto.
--- Defined.
--- Next Obligation.
---   intros y z LE. destruct (Beval z b) as [bz|] eqn:BEV.
---   erewrite Beval_increasing by eauto. destruct bz; auto.
---   destruct (Beval y b) as [[]|].
---   apply Le_trans with (x z). auto. apply Le_Join_l.
---   apply Le_trans with (x0 z). auto. apply Le_Join_r.
---   apply Join_increasing; auto.
--- Defined.
--- Next Obligation.
---   intros y z LE. apply fixpoint_Join_increasing. auto.
--- Defined.
+theorem fixpoint_join_increasing (_ : Store) (F: Store → Store) (F_mon : ∀ x y, le x y → le (F x) (F y)) (S1 S2: Store) : le S1 S2 → le (fixpoint_join' S1 F F_mon) (fixpoint_join' S2 F F_mon) := by
+  intro hyp
+  apply @fixpoint_join_smallest S1 F (by grind [wrapper]) (fixpoint_join' S2 F F_mon)
+  generalize heq : fixpoint_join' S2 F F_mon = fix2
+  have : (Le (Join S2 (F fix2)) fix2) := by
+    apply Eq_Le
+    . have := @fixpoint_join_eq S2 F (by grind [wrapper])
+      rw [←heq]
+      apply this
+  apply Le_trans
+  rotate_left
+  . apply this
+  . apply Join_increasing
+    . exact hyp
+    . grind
+
+noncomputable def Cexec' (c: com) : {F : Store → Store // ∀ x y, le x y → le (F x) (F y)} := by
+  induction c
+  case SKIP =>
+    constructor
+    case val =>
+      exact (fun S => S)
+    case property =>
+      grind
+  case ASSIGN x a =>
+    constructor
+    case val =>
+      exact (fun S => Update x (Aeval S a) S)
+    case property =>
+      intro x y hyp
+      simp
+      apply Update_increasing
+      . exact hyp
+  case SEQ c1 c2 c1_ih c2_ih =>
+    have ⟨ f₁, mon₁ ⟩ := c1_ih
+    have ⟨ f₂, mon₂ ⟩ := c2_ih
+    constructor
+    case val =>
+      exact (fun S => f₂ (f₁ S))
+    case property =>
+      grind
+  case IFTHENELSE b c1 c2 c1_ih c2_ih =>
+    have ⟨ f₁, mon₁ ⟩ := c1_ih
+    have ⟨ f₂, mon₂ ⟩ := c2_ih
+    constructor
+    case val =>
+      exact (fun S =>
+      match Beval S b with
+      | .some true => f₁ S
+      | .some false => f₂ S
+      | .none => Join (f₁ S) (f₂ S)
+      )
+    case property =>
+      intro x y hyp
+      simp
+      generalize heq : Beval y b = h
+      cases h
+      case none =>
+        simp [heq]
+        apply le_trans
+        rotate_right
+        . exact Join (f₁ x) (f₂ x)
+        rotate_left
+        . apply Join_increasing
+          . apply mon₁
+            . exact hyp
+          . apply mon₂
+            . exact hyp
+        intro id val hyp2
+        have := (Join_characterization (f₁ x) (f₂ x) id val).1 hyp2
+        split <;> grind
+      case some val =>
+        have := Beval_increasing x y hyp b val heq
+        split <;> grind
+  case WHILE b c1 c1_ih =>
+    constructor
+    case val =>
+      have ⟨ f₁, mon₁ ⟩ := c1_ih
+      exact fun S => fixpoint_join' S f₁ mon₁
+    case property =>
+      simp
+      intro x y hyp
+      apply fixpoint_join_increasing
+      . exact x
+      . exact hyp
+
+noncomputable def Cexec_Constprop (c : com) : Store → Store := (Cexec' c).val
+instance (c : com) : Monotone Store (Cexec_Constprop c) where
+  F_mon := by
+    intro x y hyp
+    exact (Cexec' c).property x y hyp
